wip

src/tls/MITLS.Repr.fst
@@ -6,9 +6,12 @@ open FStar.Integers
 
 let index (b:LP.slice 'p 'q) = i:uint_32{ i <= LP.(b.len) }
 
+let strong_parser_kind =
+    k:LP.parser_kind{LP.(k.parser_kind_subkind == Some ParserStrong)}
+
 noeq
 type repr_meta (t:Type) = {
-  parser_kind: (k:LP.parser_kind{LP.(k.parser_kind_subkind == Some ParserStrong)});
+  parser_kind: strong_parser_kind;
   parser:LP.parser parser_kind t; //erased anyway
   value: t;
 }
@@ -20,6 +23,11 @@ type repr #p #q (t:Type) (b:LP.slice p q) = {
   meta: Ghost.erased (repr_meta t)
 }
 
+
+let value #p #q (#t:Type) (#b:LP.slice p q) (r:repr t b) 
+  : GTot t
+  = (Ghost.reveal r.meta).value
+  
 let repr_p #p #q (t:Type) (b:LP.slice p q) #k (parser:LP.parser k t) =
   r:repr t b {
     let meta = Ghost.reveal r.meta in
@@ -27,16 +35,31 @@ let repr_p #p #q (t:Type) (b:LP.slice p q) #k (parser:LP.parser k t) =
     meta.parser == parser
   }
 
-let valid_pos #t #p #q (b:LP.slice p q) #k (parser:LP.parser k t) (from to:uint_32) (h:HS.mem) =
-    LP.live_slice h b /\
+let valid_pos #t #p #q (b:LP.slice p q)
+              #k (parser:LP.parser k t)
+              (from to:uint_32)
+              (h:HS.mem)
+  : prop
+  = LP.live_slice h b /\ //consequence of the next clause
     LP.valid_pos parser h b from to
 
-let valid #t #p #q (#b:LP.slice p q) (r:repr t b) (h:HS.mem)
-  : Type
+let valid' #t #p #q (#b:LP.slice p q) (r:repr t b) (h:HS.mem)
+  : prop
   = let m = Ghost.reveal r.meta in
     valid_pos b m.parser r.start_pos r.end_pos h /\
     m.value == LP.contents m.parser h b r.start_pos
 
+abstract
+let valid #t #p #q (#b:LP.slice p q) (r:repr t b) (h:HS.mem)
+  : prop
+  = valid' r h
+
+let reveal_valid ()
+  : Lemma (forall t p q (b:LP.slice p q) (r:repr t b) (h:HS.mem).
+              {:pattern (valid r h)}
+           valid r h <==> valid' r h)
+  = ()
+  
 let fp #t #p #q (#b:LP.slice p q) (r:repr t b) =
   LP.loc_slice_from_to b r.start_pos r.end_pos
   
@@ -51,3 +74,26 @@ let frame_valid #t #p #q (#b:LP.slice p q) (r:repr t b) (l:B.loc) (h0 h1:HS.mem)
     [SMTPat (valid r h1);
      SMTPat (B.modifies l h0 h1)]
   = B.modifies_buffer_from_to_elim LP.(b.base) r.start_pos r.end_pos l h0 h1
+
+open FStar.HyperStack.ST
+let mk #p #q (b:LP.slice p q) (from to:index b)
+       (#k:strong_parser_kind) #t (parser:LP.parser k t)
+  : Stack (repr_p t b parser)
+    (requires valid_pos b parser from to)
+    (ensures fun h0 r h1 ->
+      B.modifies B.loc_none h0 h1 /\
+      valid r h1)
+  = let h = get () in
+    let m =
+      let v = LP.contents parser h b from in
+      Ghost.hide ({
+        parser_kind = _;
+        parser = parser;
+        value = v
+      })
+    in
+    {
+      start_pos = from;
+      end_pos = to;
+      meta = m
+    }
